Veritas.SparseMerkleVerifier.fst
@@ -1,0 +1,175 @@
+module Veritas.SparseMerkleVerifier
+
+open FStar.Seq
+open FStar.BitVector
+open FStar.Classical
+open Veritas.SeqAux
+open Veritas.Memory
+open Veritas.Merkle
+
+//Allow the solver to unroll recursive functions at most once (fuel)
+//Allow the solver to invert inductive definitions at most once (ifuel)
+#push-options "--max_fuel 1 --max_ifuel 1 --initial_fuel 1 --initial_ifuel 1"
+
+(* 
+ * The verifier consumes a log that consists of memory operations and 
+ * additional "proof" objects and returns success of failure; we prove
+ * that if the verifier returns success, then the underlying memory 
+ * operations are read-write consistent 
+ *)
+
+(* Each entry of the verifier log *)
+type verifier_log_entry = 
+  | MemoryOp: o:memory_op -> verifier_log_entry
+  | Add: a:merkle_addr -> v:sp_merkle_payload -> a':merkle_addr -> verifier_log_entry
+  | Evict: a:merkle_addr -> a':merkle_addr -> verifier_log_entry
+
+type verifier_log = seq verifier_log_entry
+
+(* index in the verifier log *)
+type vl_index (l:verifier_log) = seq_index l
+
+(* is the i'th operation an evict *)
+let is_evict (l:verifier_log) (i:vl_index l): Tot bool =
+  Evict? (index l i)
+
+(* evicted address for an evict operation *)
+let evict_addr (l:verifier_log) (i:vl_index l{is_evict l i}): Tot merkle_addr = 
+  Evict?.a (index l i)
+
+(* ancestor recording the evicted nodes hashes *)
+let evict_ancestor (l:verifier_log) (i:vl_index l{is_evict l i}): Tot merkle_addr = 
+  Evict?.a' (index l i)
+
+(* is the ith operation an add *)
+let is_add (l:verifier_log) (i:vl_index l) = 
+  Add? (index l i)
+
+(* added address for an add operation *)
+let add_addr (l:verifier_log) (i:vl_index l{is_add l i}): Tot merkle_addr = 
+  Add?.a (index l i)
+
+(* added payload for an add operation *)
+let add_payload (l:verifier_log) (i:vl_index l {is_add l i}): Tot sp_merkle_payload =
+  Add?.v (index l i)
+
+let add_ancestor (l:verifier_log) (i:vl_index l {is_add l i}): Tot merkle_addr = 
+  Add?.a' (index l i)
+
+(* is the ith operation a memory operation? *)
+let is_memory_op (l:verifier_log) (i:vl_index l): Tot bool = MemoryOp? (index l i)
+
+(* memory op for an memory_op index *)
+let memory_op_at (l:verifier_log) (i:vl_index l{is_memory_op l i}) = MemoryOp?.o (index l i)
+
+(* is the i'th operation a write operation *)
+let is_write_op (l:verifier_log) (i:vl_index l): Tot bool = 
+  is_memory_op l i && Write? (memory_op_at l i)
+
+(* written value for a write operation *)
+let written_value (l:verifier_log) (i:vl_index l{is_write_op l i}): Tot payload = 
+  Write?.v (memory_op_at l i)
+
+(* is the ith operation a read operation *)
+let is_read_op (l:verifier_log) (i:vl_index l): Tot bool = 
+  is_memory_op l i && Read? (memory_op_at l i)
+
+(* read value for a read operation *)
+let read_value (l:verifier_log) (i:vl_index l{is_read_op l i}): Tot payload = 
+  Read?.v (memory_op_at l i)
+
+(* Verifier cache of a subset of merkle_addr, merkle_payloads *)
+type verifier_cache = (a:merkle_addr) -> option (sp_merkle_payload_of_addr a)
+
+(* Does the cache contain a merkle addr? *)
+let cache_contains (vc:verifier_cache) (a:merkle_addr): Tot bool = 
+  Some? (vc a)
+
+(* Lookup the payload of an address in cache *)
+let cached_payload (cache:verifier_cache) (a:merkle_addr{cache_contains cache a}): Tot (sp_merkle_payload_of_addr a) =
+  Some?.v (cache a)
+
+(* 
+ * Update the cache. This is a pure update function that requires 
+ * that cache contain an entry for the merkle address as a precondition
+ *)
+let cache_update (cache:verifier_cache) 
+                 (a:merkle_addr{cache_contains cache a}) 
+                 (v:sp_merkle_payload_of_addr a): 
+  Tot (cache':verifier_cache{cache_contains cache' a}) = 
+  fun a' -> if a' = a then Some v else cache a'
+
+(* 
+ * Update the cache to reflect a memory write, which translates to updating 
+ * the leaf merkle node in the cache. This is a pure update function and we 
+ * require the cache to contain an entry for the merkle addr as a precondition
+ *)
+let cache_apply (cache:verifier_cache)
+                (o:memory_op{Write? o && 
+                             cache_contains cache (addr_to_merkle_leaf (address_of o))})
+  : Tot (vc':verifier_cache{cache_contains vc' (addr_to_merkle_leaf (address_of o))}) =
+  match o with
+  | Read _ _ -> cache
+  | Write a v -> cache_update cache (addr_to_merkle_leaf a) (SMkLeaf v)
+  
+(* Add a merkle_addr, payload to cache *)
+let cache_add (cache:verifier_cache)
+              (a:merkle_addr {not (cache_contains cache a)}) 
+              (v:sp_merkle_payload_of_addr a) 
+  : Tot (cache':verifier_cache {cache_contains cache' a}) =
+  fun a' -> if a' = a then Some v else cache a'
+
+(* Evict a merkle_addr from cache *)
+let cache_evict (cache:verifier_cache) 
+                (a:merkle_addr{cache_contains cache a}) 
+  : Tot verifier_cache = 
+  fun a' -> if a' = a then None else cache a'
+
+(* Verifier state is the cache if valid *)
+noeq type verifier_state = 
+  | Failed: verifier_state 
+  | Valid: vc:verifier_cache -> verifier_state
+
+let is_hash_at_ancestor_correct (cache:verifier_cache)
+                                (a:merkle_non_root_addr)
+                                (v:sp_merkle_payload_of_addr a)
+                                (a': merkle_addr): Tot bool = 
+  (* check a' is an ancestor of a *)
+  if not (is_desc a a') then false
+  (* check a' is in the cache *)
+  else if not (cache_contains cache a') then false  
+  else
+    let v' = cached_payload cache a' in
+    
+    admit()
+
+let verifier_step (e:verifier_log_entry) (vs:verifier_state): Tot verifier_state = 
+  (* propagate failures *)
+  if (Failed? vs) then Failed
+  else
+    let cache = (Valid?.vc vs) in
+    match e with
+    (* Memory operation *)
+    | MemoryOp o ->
+        let optPayload = cache (addr_to_merkle_leaf (address_of o)) in
+        (* If the address is not in our cache, verification fails *)
+        if (None? optPayload) then Failed
+        else (
+          let payload = Some?.v optPayload in
+          match o with
+          (* For reads, the value read should correspond to the value in the cache *)
+          | Read _ v -> if v = SMkLeaf?.value payload then vs else Failed            
+          (* For writes, update the cache to reflect the write *)
+          | Write a v -> Valid (cache_apply cache o))
+     | Add a v a' -> 
+         (* Check cache contains merkle addr a *)
+         if cache_contains cache a then Failed 
+         (* Root is never added *)
+         else if is_merkle_root a then Failed
+         (* Check the payload type corresponds to leaf/internal ness of address a *)
+         else if not (is_sp_payload_of_addr a v) then Failed 
+         (* check the hash of a v is stored at ancestor a' *)
+         else if not (is_hash_at_ancestor_correct cache a v a') then Failed 
+         (* All checks passed - add (a,v) to the cache *)
+         else Valid (cache_add cache a v)
+     | Evict a a' -> admit()
